Isabelle2/LinorderOption.thy
@@ -1,0 +1,36 @@
+theory LinorderOption
+imports Main
+begin
+section {* nat option as a linear order *}
+
+fun less_eq_o where 
+  "less_eq_o None _ = True"
+| "less_eq_o (Some x) None = False"
+| "less_eq_o (Some x) (Some y) = (x \<le> y)"
+
+fun less_o where
+  "less_o None None = False" 
+| "less_o None _ = True"
+| "less_o (Some x) None = False"
+| "less_o (Some x) (Some y) = (x < y)"
+
+instantiation option :: (linorder) linorder
+begin
+
+definition less_eq_def:"o1 \<le> o2 = less_eq_o o1 o2"
+definition less_def:"o1 < o2 = less_o o1 o2"
+
+instance 
+apply(intro_classes)
+apply (auto simp add:less_eq_def less_def)
+apply (metis le_cases less_eq_o.elims(3) less_o.elims(2) less_o.simps(1) less_o.simps(2) not_le option.inject)
+apply (metis less_eq_o.elims(2) less_o.elims(2) less_o.simps(1) less_o.simps(2) not_le option.inject)
+apply (metis less_eq_o.elims(3) less_o.simps(2) less_o.simps(4) not_le)
+apply (metis less_eq_o.elims(3) less_eq_o.simps(1) option.sel order_refl)
+apply (smt less_eq_o.elims(2) less_eq_o.elims(3) less_o.simps(1) less_o.simps(2) option.inject order_trans)
+apply (metis dual_order.antisym less_eq_o.elims(2) less_eq_o.simps(2) option.inject)
+by (metis le_cases less_eq_o.elims(3) option.discI option.inject)
+
+end
+
+end
